Consider the proposition~\eqref{prop:binomial-decomposition}.
For integers $n\geq 0, \; r \geq 0, \; m\geq 0$, we have
\begin{align*}
  n \binom{n+r}{m} = (m+1) \binom{n+r}{m+1} - (r-m) \binom{n+r}{m}
\end{align*}
For that case,
the extraction property of binomial coefficients fits perfectly.
\begin{lemma} [Extraction]
  \begin{align*}
    \binom{n}{k+1} = \frac{n-k}{k+1} \binom{n}{k}
  \end{align*}
\end{lemma}
Thus,
\begin{align*}
  &n \binom{n+r}{m}
  = (m+1) \binom{n+r}{m+1} - (r-m) \binom{n+r}{m} \\
  &= m \binom{n+r}{m+1} + \binom{n+r}{m+1} - r \binom{n+r}{m} + m \binom{n+r}{m}
\end{align*}
Now we can notice that
\begin{align*}
  \binom{n+r}{m+1} = \frac{n+r-m}{m+1} \binom{n+r}{m},
\end{align*}
by extraction.
Thus,
\begin{align*}
  n \binom{n+r}{m}
  &= m \frac{n+r-m}{m+1} \binom{n+r}{m} + \frac{n+r-m}{m+1} \binom{n+r}{m} - r \binom{n+r}{m} + m \binom{n+r}{m}
\end{align*}
By moving binomial coefficient $\binom{n+r}{m}$ out of the brackets, we get
\begin{align*}
  n \binom{n+r}{m}
  &= \binom{n+r}{m} \left[ m \frac{n+r-m}{m+1} + \frac{n+r-m}{m+1} - r + m \right] \\
  &= \binom{n+r}{m} \left[ (m+1) \frac{n+r-m}{m+1} - r + m \right]
\end{align*}
Therefore, it is indeed true that for integers $n\geq 0, \; r \geq 0, \; m\geq 0$
\begin{align*}
  n \binom{n+r}{m} = (m+1) \binom{n+r}{m+1} - (r-m) \binom{n+r}{m}
\end{align*}
This completes the proof. \qed
